

1. (20 points) (a) Find the solution of the initial boundary value problem for the one dimensional wave equation with homogeneous Neumann boundary condition

$$\begin{cases} u_{tt} - c^2 u_{xx} = 0 & 0 < x < L, t > 0 \\ u(x, 0) = g(x), u_t(x, 0) = h(x) & 0 < x < L \\ u_x(0, t) = u_x(L, t) = 0 & t > 0. \end{cases}$$

Please include the details as we did for the homogeneous Dirichlet boundary condition during the lecture.

- (b) Consider the initial boundary value problem

$$\begin{cases} u_{tt} - u_{xx} = 0 & 0 < x < \pi, t > 0 \\ u(x, 0) = x^2, u_t(x, 0) = 0 & 0 < x < \pi \\ u_x(0, t) = u_x(\pi, t) = 0 & t > 0. \end{cases}$$

Find a Fourier series solution.

a) Assume $u(x, t) = XT$

$$XT'' - c^2 X''T = 0$$

$$\frac{X''}{X} = \frac{T''}{c^2 T} \Rightarrow T \text{ and } X \text{ are constants}$$

$$X'' = \lambda X$$

$\lambda > 0$ $X = c_1 e^{\sqrt{\lambda}x} + c_2 e^{-\sqrt{\lambda}x}$

$$X' = c_1 \sqrt{\lambda} e^{\sqrt{\lambda}x} - c_2 \sqrt{\lambda} e^{-\sqrt{\lambda}x}$$

$$X'(0) = 0 = \sqrt{\lambda}(c_1 - c_2)$$

$$\Rightarrow c_1 = c_2 \text{ because } \lambda > 0$$

$$X'(L) = \sqrt{\lambda}c_1(e^{\sqrt{\lambda}L} - e^{-\sqrt{\lambda}L}) = 0$$

$$\text{Since } \lambda > 0, L > 0 \quad e^{\sqrt{\lambda}L} - e^{-\sqrt{\lambda}L} \neq 0 \Rightarrow c_1 = 0$$

$$\Rightarrow u(x, t) = 0$$

$\lambda = 0$ $X = c_1 + c_2 X$

$$X'(0) = 0 = c_2$$

$$X = c_1 \Rightarrow u(x, t) = u(t) = c_1 T(t)$$

$\lambda < 0$ $X = c_1 \cos(\sqrt{-\lambda}x) + c_2 \sin(\sqrt{-\lambda}x)$

$$X' = -\sqrt{-\lambda}c_1 \sin(\sqrt{-\lambda}x) + \sqrt{-\lambda}c_2 \cos(\sqrt{-\lambda}x)$$

$$X'(0) = 0 = 0 + \sqrt{\lambda} C_2 \Rightarrow C_2 = 0$$

$$X'(L) = 0 = \sqrt{-\lambda} C_1 \sin(\sqrt{-\lambda} L)$$

$$\Rightarrow \sqrt{-\lambda} L = k\pi$$

$$\lambda = -\frac{k^2 \pi^2}{L^2}$$

$$X_k = C_k \cos \frac{k\pi x}{L}$$

$$T'' = \lambda c^2 T$$

$$\lambda = 0 \quad T = C_2 + C_3 t$$

$$u(x,t) = u(t) = C_1 (C_2 + C_3 t) \quad C_1 C_2 = A_0 \quad C_1 C_3 = B_0$$

$$\lambda > 0 \quad u(x,t) = 0 \quad T(t) = 0$$

$$\lambda < 0 \quad \lambda = -\frac{k^2 \pi^2}{L^2} \Rightarrow T_k = a_k \cos \frac{k\pi c t}{L} + b_k \sin \frac{k\pi c t}{L}$$

$$\text{Let } a_k C_k = A_k \quad b_k C_k = B_k$$

$$u(x,t) = B_0 t + A_0 + \sum_{k=1}^{\infty} \cos \frac{k\pi x}{L} (A_k \cos \frac{k\pi c t}{L} + B_k \sin \frac{k\pi c t}{L})$$

$$\dot{u}(x,t) = B_0 + \sum_{k=1}^{\infty} \frac{k\pi c}{L} \cos \frac{k\pi x}{L} (B_k \cos \frac{k\pi c t}{L} - A_k \sin \frac{k\pi c t}{L})$$

$$u(x,0) = A_0 + \sum_{k=1}^{\infty} A_k \cos \frac{k\pi x}{L} = g(x)$$

even expansion of g

$$A_0 = \frac{1}{L} \int_0^L g(x) dx \quad A_k = \frac{2}{L} \int_0^L g(x) \cos \frac{k\pi x}{L} dx$$

$$\dot{u}(x,0) = h(x) = B_0 + \sum_{k=1}^{\infty} B_k \frac{k\pi c}{L} \cos \frac{k\pi x}{L}$$

even expansion of h

$$B_0 = \frac{1}{L} \int_0^L h(x) dx \quad B_k = \frac{2}{k\pi c} \int_0^L h(x) \cos \frac{k\pi x}{L} dx$$

$$\therefore u(x,t) = B_0 t + A_0 + \sum_{k=1}^{\infty} \cos \frac{k\pi x}{L} (A_k \cos \frac{k\pi c t}{L} + B_k \sin \frac{k\pi c t}{L})$$

$$\text{Where } A_0 = \frac{1}{L} \int_0^L g(x) dx \quad A_k = \frac{2}{L} \int_0^L g(x) \cos \frac{k\pi x}{L} dx$$

$$B_0 = \frac{1}{L} \int_0^L h(x) dx \quad B_k = \frac{2}{k\pi c} \int_0^L h(x) \cos \frac{k\pi x}{L} dx$$

$$b) \quad g(x) = x^2 \quad h(x) = 0 \quad L = \pi \quad c = 1$$

From part a

$$n = 1, 2, 3, \dots, \infty$$

From part a

$$u(x,t) = \frac{1}{\pi} \int_0^\pi x^2 dx + \sum_{k=1}^{\infty} \cos kx \left(\frac{1}{\pi} \int_0^\pi x^2 \cos kx dx \right) (\cos kt + 0)$$

$$= \frac{\pi^3}{3} + \sum_{k=1}^{\infty} \cos kx \cos kt \frac{4(-1)^k}{k^2}$$

(%i4) integrate(x^2,x,0,pi)/pi;

(%o4) $\frac{\pi^2}{3}$

(%i6) declare(k,integer);

(%o6) done

(%i7) 2*integrate(x^2*cos(k*x),x,0,pi)/pi;

(%o7) $\frac{4(-1)^k}{k^2}$

2. (20 points) Find the solution of the initial boundary value problem for the one dimensional homogeneous wave equation with nonhomogeneous Dirichlet boundary condition

$$\begin{cases} u_{tt} - u_{xx} = 0 & 0 < x < \pi, t > 0 \\ u(x,0) = 0, u_t(x,0) = 0 & 0 < x < \pi \\ u(0,t) = u(\pi,t) = 2t^2 - 3 & t > 0. \end{cases}$$

(Hint: As we did during the lecture, first convert it into a nonhomogeneous wave equation with homogeneous Dirichlet boundary condition. Then you can decompose the problem into a homogeneous equation with homogeneous Dirichlet boundary condition, for which we already have the solution from the lecture, and another part of a nonhomogeneous equation with zero initial condition, for which you can use Duhamel's principle. When you solve the "w" part in Duhamel's principle, you will find that w satisfies a homogeneous equation with homogeneous Dirichlet boundary condition, for which we again have solution.)

Consider

$$\tilde{u}(x,t) = 2t^2 - 3 + \frac{x}{\pi} (2t^2 - 3 - 2t^2 + 3)$$

$$= 2t^2 - 3$$

$$\tilde{u}(0,t) = \tilde{u}(\pi,t) = 2t^2 - 3$$

$$\text{Let } v = u - \tilde{u}$$

$$\text{It follows } \begin{cases} v_{tt} - v_{xx} = \overbrace{u_{tt} - u_{xx}}^0 - 4 = -4 & 0 < x < \pi, t > 0 \\ v(x,0) = 0 - 3 = -3 & v_t(x,0) = 0 - 0 \\ v(0,t) = 2t^2 - 3 - (2t^2 - 3) = 0 & \\ v(\pi,t) = 2t^2 - 3 - (2t^2 - 3) = 0 & t > 0 \end{cases}$$

Let $v = v_1 + v_2$ where

$$v_1: v_1 - \lambda_1 v_1 = 0 \quad 0 < x < \pi, t > 0 \quad \lambda_1 = \lambda_2 = \dots = \lambda_n = -4 \quad 0 < x < \pi$$

Let $V = V_1 + V_2$ where

$$\begin{aligned} \underline{V_1} \quad & \partial_t V_1 - \partial_{xx} V_1 = 0 \quad 0 < x < \pi, t > 0 \\ & V_1(x, 0) = 3 \quad \partial_t V_1(x, 0) = 0 \quad 0 < x < \pi \\ & V_1(0, t) = V_1(\pi, t) = 0 \quad t > 0 \end{aligned}$$

$$\begin{aligned} \underline{V_2} \quad & \partial_t V_2 - \partial_{xx} V_2 = -4 \quad 0 < x < \pi, t > 0 \\ & V_2(x, 0) = \partial_t V_2(x, 0) = 0 \quad 0 < x < \pi \\ & V_2(0, t) = V_2(\pi, t) = 0 \quad t > 0 \end{aligned}$$

$$C=1 \quad L=\pi \quad g(x)=3 \quad h(x)=0$$

$$\underline{V_1} \quad V_1(x, t) = \sum_{k=1}^{\infty} \sin kx [a_k \cos kt]$$

$$a_k = \frac{2}{\pi} \int_0^{\pi} 3 \sin kx dx = \frac{6}{\pi} \left(\frac{1 - (-1)^k}{k} \right)$$

(%i6) declare(k, integer);

(%o6) done

(%i24) 2-integrate(3*sin(k*x), x, 0, pi)/pi;

(%o24) $6 \left(\frac{1}{k} - \frac{(-1)^k}{k} \right) / \pi$

$$\underline{V_2} \quad \forall s > 0 \quad w(x, t; s) \text{ solves } \begin{cases} \partial_t w - \partial_{xx} w = 0 & 0 < x < \pi, t > 0 \\ w(x, s; s) = 0 & 0 < x < \pi \\ w_t(x, s; s) = -4 & 0 < x < \pi \\ w(0, t; s) = w(\pi, t; s) = 0 & t > 0 \end{cases}$$

By Duhamel's principle

$$\text{and } V_2(x, t) = \int_0^t w(x, t; s) ds$$

$$C=1 \quad L=\pi \quad h(x)=-4 \quad g(x)=0$$

$$V_2(x, t) = \int_0^t \sum_{k=1}^{\infty} \sin kx b_k \sin ks ds$$

$$b_k = \frac{2}{k\pi} \int_0^{\pi} -4 \sin kx dx = \frac{-8}{\pi} \left(\frac{1 - (-1)^k}{k^2} \right)$$

2-integrate(-4*sin(k*x), x, 0, pi)/(k*pi);

$- \left(\frac{8}{\pi k} \left(\frac{1}{k} - \frac{(-1)^k}{k} \right) \right)$

$$V_2(x, t) = \int_0^t \sum_{k=1}^{\infty} \frac{-8}{\pi k^2} (1 - (-1)^k) \sin kx \sin ks ds$$

) integrate(sin(k*x), x, 0, t);

Is t positive, negative or zero? **positive;**

$$= \sum_{k=1}^{\infty} \frac{8}{\pi k^3} (1 - (-1)^k) \sin kx (\cos kt - 1)$$

5) $\frac{1}{k} - \frac{\cos(kt)}{k}$

$$V = \sum_{k=1}^{\infty} \sin kx (1 - (-1)^k) \left(\frac{6}{\pi k} \cos kt + \frac{8}{\pi k^3} (\cos kt - 1) \right)$$

$$\therefore u = 2t^2 - 3 + \sum_{k=1}^{\infty} \sin kx (1 - (-1)^k) \left(\frac{6}{\pi k} \cos kt + \frac{8}{\pi k^3} (\cos kt - 1) \right)$$

3. (20 points) Find the solution of the following initial value problems. You can use the Kirchhoff's formula directly. (Hint: you can use the spherical coordinator. You should be able to compute the integral explicitly.)

(a)

$$\begin{cases} u_{tt} - \Delta u = 0 & x = (x_1, x_2, x_3) \in \mathbb{R}^3, t > 0 \\ u(x, 0) = 0, u_t(x, 0) = x_1^2 + x_2^2 + x_3^2 & x = (x_1, x_2, x_3) \in \mathbb{R}^3 \end{cases}$$

(b)

$$\begin{cases} u_{tt} - \Delta u = 0 & x = (x_1, x_2, x_3) \in \mathbb{R}^3, t > 0 \\ u(x, 0) = x_1^2 + x_2^2, u_t(x, 0) = 0 & x = (x_1, x_2, x_3) \in \mathbb{R}^3 \end{cases}$$

$$u(x, t) = \int_{\partial B_t(x)} (g(y) + \nabla g(y) \cdot (y - x) + th(y)) dS_y$$

a) $g(x) = 0 \quad h(x) = x_1^2 + x_2^2 + x_3^2$

a) $g(x) = 0$ $h(x) = x_1^2 + x_2^2 + x_3^2$

$$\begin{aligned} u(x, t) &= \int_{\partial B_t(0)} g(y) + \nabla g(y) \cdot (y - x) dS_y \quad y_i = x_i + t z_i \\ &= \frac{t}{4\pi} \int_{\partial B_t(0)} (x_1 + t z_1)^2 + (x_2 + t z_2)^2 + (x_3 + t z_3)^2 dS_z \\ &= \frac{t}{4\pi} \int_{\partial B_t(0)} x_1^2 + x_2^2 + x_3^2 + 2t(x_1 z_1 + x_2 z_2 + x_3 z_3) + t^2(z_1^2 + z_2^2 + z_3^2) dS_z \\ &= \frac{t}{4\pi} (4\pi(x_1^2 + x_2^2 + x_3^2) + 0 + 4\pi t^2) \end{aligned}$$

Note $\int_{\partial B_t(0)} z_i dS = 0$ by symmetry and $\int_{\partial B_t(0)} z_i^2 dS = \frac{4\pi}{3} t^2$
 $= t(x_1^2 + x_2^2 + x_3^2 + t^2)$

b) $g(x) = x_1^2 + x_2^2$ $h(x) = 0$

$$\begin{aligned} u(x, t) &= \int_{\partial B_t(0)} g(y) + \nabla g(y) \cdot (y - x) dS_y \quad y_i = x_i + t z_i \\ &= \frac{1}{4\pi} \int_{\partial B_t(0)} (x_1 + t z_1)^2 + (x_2 + t z_2)^2 + [2(x_1 + t z_1), 2(x_2 + t z_2), 0] \begin{bmatrix} t z_1 \\ t z_2 \\ t z_3 \end{bmatrix} dS_z \\ &= \frac{1}{4\pi} \int_{\partial B_t(0)} x_1^2 + x_2^2 + 2t(x_1 z_1 + x_2 z_2) + t^2(z_1^2 + z_2^2) \\ &\quad + 2t(x_1 z_1 + x_2 z_2) + t^2(z_1^2 + z_2^2) dS_z \end{aligned}$$

Similarly to part a,

$$\begin{aligned} \int_{\partial B_t(0)} z_i dS &= 0 \text{ by symmetry and } \int_{\partial B_t(0)} z_i^2 dS = \frac{4\pi}{3} t^2 \\ &= \frac{1}{4\pi} (4\pi(x_1^2 + x_2^2) + 0 + \cancel{8\pi t^2} \frac{8\pi}{3}) \\ &= x_1^2 + x_2^2 + 2t^2 \end{aligned}$$